Veritas.SeqAux.fsti
@@ -1,0 +1,66 @@
+module Veritas.SeqAux
+
+open FStar.Seq 
+
+(* Legitimate values of an index of a sequence *)
+type seq_index (#a:Type) (s:seq a) = i:nat{i < length s}
+
+(* Prefix of a sequence *)
+val prefix (#a:Type) (s:seq a) (i:nat{i <= length s}): Tot (s':seq a{length s' = i})
+
+val lemma_prefix_index (#a:Type) (s:seq a) (i:nat{i <= length s}) (j:nat{j < i}):
+  Lemma (requires (True))
+        (ensures (index (prefix s i) j == index s j))
+
+(* Suffix of a sequence *)
+val suffix (#a:Type) (s:seq a) (i:nat{i <= length s}): Tot (s':seq a{length s' = i})
+
+val lemma_suffix_index (#a:Type) (s:seq a) (i:nat{i <= length s}) (j:nat{j < i}):
+  Lemma (requires (True))
+        (ensures (index (suffix s i) j == index s (length s - i + j)))
+
+(* Subsequence of s obtained by applying a filter *)
+val filter (#a:eqtype) (f:a -> bool) (s:seq a): Tot (seq a)
+
+(* Mapping from original seq to filtered subseq for satisfying indexes *)
+val filter_index_map (#a:eqtype) (f:a -> bool) (s:seq a) (i:seq_index s{f (index s i)}):
+  Tot (j:seq_index (filter f s){index s i = index (filter f s) j})
+
+(* filter_index_map is injective *)
+val filter_index_map_monotonic (#a:eqtype) (f:a -> bool) (s:seq a) 
+  (i:seq_index s)(j:seq_index s{j > i}):
+  Lemma (requires (f (index s i) && f (index s j)))
+        (ensures (filter_index_map f s i < filter_index_map f s j))  
+
+(* Inverse mapping from filtered subseq to satisfying indexes *)
+val filter_index_inv_map (#a:eqtype) (f:a -> bool) (s:seq a) 
+  (i:seq_index (filter f s)): 
+  Tot (j:seq_index s{f (index s j) /\ filter_index_map f s j = i})
+
+(* The index of the last entry that satisfies a given property *)
+val last_index_opt (#a:eqtype) (f:a -> bool) (s:seq a):
+  Tot (option (i:seq_index s{f (index s i)}))
+
+(* There exists some element satisfying f if there exists last_index *)
+let exists_sat_elems (#a:eqtype) (f:a -> bool) (s:seq a) = 
+  Some? (last_index_opt f s)
+
+(* The index of the last entry when we know there exists such entry *)
+let last_index (#a:eqtype) (f:a -> bool) (s:seq a{exists_sat_elems f s}) =
+  Some?.v (last_index_opt f s)
+
+(* Any index beyond last index does not satisfy f *)
+val lemma_last_index_correct1 (#a:eqtype) (f:a -> bool) (s:seq a) (i:seq_index s):
+  Lemma (requires (exists_sat_elems f s /\ i > last_index f s))
+        (ensures (not (f (index s i))))
+
+(* Any witness satisfying f implies last_index exists *)
+val lemma_last_index_correct2 (#a:eqtype) (f:a -> bool) (s:seq a) (i:seq_index s):
+  Lemma (requires (f (index s i)))
+        (ensures (exists_sat_elems f s /\ last_index f s >= i))
+
+(* Taking the prefix of a sequence upto last_index does not alter last_index *)
+val lemma_last_index_prefix (#a:eqtype) (f:a -> bool) (s:seq a):
+  Lemma (requires (exists_sat_elems f s))
+        (ensures (exists_sat_elems f (prefix s ((last_index f s) + 1)) /\
+                  last_index f s = last_index f (prefix s ((last_index f s) + 1))))
