Makefile
@@ -1,0 +1,44 @@
+.PHONY: verify clean
+
+# List the files that should be verified by verify-extra and verify-all
+EXTRA=
+
+# List the files that should NOT be verified at all
+FLAKY=
+
+# List the files that should be verified by verify-core and verify-all
+# Those files are the roots from where all dependencies are computed
+FSTAR_FILES := Veritas.SeqAux.fsti Veritas.SeqAux.fst
+
+USE_EXTRACTED_INTERFACES=--use_extracted_interfaces true
+
+OTHERFLAGS+=$(USE_EXTRACTED_INTERFACES)
+
+# 271: theory symbols in smt patters
+WARN_ERROR=--warn_error -271
+VALIDITY_AXIOMS?=--smtencoding.valid_intro true --smtencoding.valid_elim true
+OTHERFLAGS+=$(WARN_ERROR) --z3cliopt 'timeout=600000' $(VALIDITY_AXIOMS)
+
+FSTAR=fstar.exe $(OTHERFLAGS)
+
+# A place to put all the emitted .ml files
+OUTPUT_DIRECTORY ?= _output
+
+MY_FSTAR=$(FSTAR) --cache_checked_modules --odir $(OUTPUT_DIRECTORY)
+
+# a.fst.checked is the binary, checked version of a.fst
+%.fst.checked: %.fst
+	$(MY_FSTAR) $*.fst
+	touch $@
+
+# a.fsti.checked is the binary, checked version of a.fsti
+%.fsti.checked: %.fsti
+	$(MY_FSTAR) $*.fsti
+	touch $@
+
+LowStar.Printf.fst.checked: USE_EXTRACTED_INTERFACES=
+
+verify: $(addsuffix .checked, $(FSTAR_FILES))
+
+clean:
+	rm -rf *.checked
